Word: more laws

bedrock2/src/Word/Naive.v
@@ -6,29 +6,6 @@ Require Import bedrock2.Word. Import word.
 Local Open Scope Z_scope.
 
 (* TODO: move me? *)
-(* from https://github.com/coq/coq/pull/8062/files#diff-c73fff6c197eb53a5ca574b51e21bf82 *)
-Require Import Lia.
-Module Z.  Lemma mod_0_r_ext x y : y = 0 -> x mod y = 0.
-  Proof. intro; subst; destruct x; reflexivity. Qed.
-  Lemma div_0_r_ext x y : y = 0 -> x / y = 0.
-  Proof. intro; subst; destruct x; reflexivity. Qed.
-
-  Ltac div_mod_to_quot_rem_generalize x y :=
-    pose proof (Z.div_mod x y);    pose proof (Z.mod_pos_bound x y);
-    pose proof (Z.mod_neg_bound x y);    pose proof (div_0_r_ext x y);
-    pose proof (mod_0_r_ext x y);    let q := fresh "q" in
-    let r := fresh "r" in    set (q := x / y) in *;
-    set (r := x mod y) in *;
-    clearbody q r.  Ltac div_mod_to_quot_rem_step :=
-    match goal with    | [ |- context[?x / ?y] ] => div_mod_to_quot_rem_generalize x y
-    | [ |- context[?x mod ?y] ] => div_mod_to_quot_rem_generalize x y    | [ H : context[?x / ?y] |- _ ] => div_mod_to_quot_rem_generalize x y
-    | [ H : context[?x mod ?y] |- _ ] => div_mod_to_quot_rem_generalize x y    end.
-  Ltac div_mod_to_quot_rem := repeat div_mod_to_quot_rem_step.
-End Z.
-Ltac mia := Z.div_mod_to_quot_rem; nia.
-
-
-(* TODO: move me? *)
 Definition minimize_eq_proof{A: Type}(eq_dec: forall (x y: A), {x = y} + {x <> y}){x y: A}    (pf: x = y): x = y :=
   match eq_dec x y with
   | left p => p
@@ -38,19 +15,19 @@ Definition minimize_eq_proof{A: Type}(eq_dec: forall (x y: A), {x = y} + {x <> y
 Section WithWidth.
   Context {width : Z}.
   Let wrap_value z := z mod (2^width).
+  Let swrap_value z := wrap_value (z + 2 ^ (width - 1)) - 2 ^ (width - 1).
   Record rep := mk { unsigned : Z ; _unsigned_in_range : wrap_value unsigned = unsigned }.
 
   Context {width_nonneg : Z.lt 0 width}.
 
   Lemma wrap_value_wrap_value z : wrap_value (wrap_value z) = wrap_value z.
     cbv [wrap_value]. rewrite Z.mod_mod. reflexivity.
-    eapply Z.pow_nonzero; [congruence | lia ].
+    eapply Z.pow_nonzero; [congruence | Lia.lia ].
   Qed.
 
   Definition wrap (z:Z) : rep :=
     mk (wrap_value z) (minimize_eq_proof Z.eq_dec (wrap_value_wrap_value z)).
-  Definition signed w :=
-    unsigned w mod 2^(width-1) - 2^(width-1) * (unsigned w / 2^(width-1)).
+  Definition signed w := swrap_value (unsigned w).
 
   Definition word : word.word width := {|
     word.rep := rep;
@@ -66,7 +43,7 @@ Section WithWidth.
     and x y := wrap (Z.land (unsigned x) (unsigned y));
     xor x y := wrap (Z.lxor (unsigned x) (unsigned y));
     not x := wrap (Z.lnot (unsigned x));
-    ndn x y := wrap (Z.land (unsigned x) (Z.lnot (unsigned y)));
+    ndn x y := wrap (Z.ldiff (unsigned x) (unsigned y));
 
     mul x y := wrap (Z.mul (unsigned x) (unsigned y));
     mulhss x y := wrap (Z.mul (signed x) (signed y) / 2^width);
@@ -99,20 +76,8 @@ Section WithWidth.
 
   Lemma signed_of_Z z : signed (wrap z) = wrap_value (z + 2 ^ (width - 1)) - 2 ^ (width - 1).
   Proof.
-    cbv [unsigned signed wrap wrap_value].
-    set (M := 2 ^ (width - 1)).
-    assert (0 < M) by (change 0 with (2^(-1)); eapply Z.pow_lt_mono_r; lia).
-    assert (0 < 2*M) by lia.
-    replace (2^width) with (2*M) in * by
-        (subst M; rewrite <-Z.pow_succ_r, Z.sub_1_r, Z.succ_pred; nia).
-    clearbody M.
-    rewrite (Z.add_mod z M (2*M)) by lia.
-    assert (M/(2 * M)=0) as H2M by mia;
-      replace (M mod (2 * M)) with M by mia; clear H2M.
-    set (X := z mod (2*M));
-      destruct (ltac:(subst X; mia):(0 <= X < M \/ M <= X < 2*M)); clearbody X.
-    { assert (X/M = 0) by mia; assert ((X + M) / (2 * M) = 0); mia. }
-    { assert (X/M = 1) by mia; assert ((X + M) / (2 * M) = 1); mia. }
+    cbv [unsigned signed wrap wrap_value swrap_value].
+    rewrite Zdiv.Zplus_mod_idemp_l; auto.
   Qed.
 
   Lemma ok : word.ok word.
